Completed part 3 for Polynomials

take-home1/polynomials-submission.dfy
@@ -39,45 +39,97 @@ lemma polyval_slicing(a : seq<int>, x: int, i:nat)
     
 }
 
-function polyseg(a: seq<int>, x: int, lo: nat, hi: nat) : int
-requires hi >= lo && hi <= |a|
-decreases hi - lo
+lemma PowProperty(x: int, a: nat, b:nat) 
+    requires b >= a
+    ensures pow(x, b) == pow(x, a) * pow(x, b - a)
 {
-    if |a| == 0
-    then 
-        0
-    else if lo == hi
-    then 
-        0
-    else 
-        polyseg(a, x, lo, hi - 1) + pow(x, hi - 1) * a[hi - 1]
-}
-
-lemma polyseg_equals_polyval_general(a: seq<int>, x:int, d: nat)
-    requires 0 <= d <= |a|
-    ensures polyval(a[..d], x) == polyseg(a, x, 0, d)
-{
-    if d == 0 {
-        assert polyval(a[..d], x) == 0;
-        assert polyseg(a[..d], x, 0, d) == 0;
+    if b == a {
+        assert pow(x, b - a) == 1;
+        assert pow(x, b) == pow(x, a);
+        assert pow(x, b) == pow(x, a) * pow(x, b - a);
     } else {
-        var d' := d - 1;
-        assert 0 <= d' <= |a|;
-        polyval_slicing(a, x, d);
-        assert polyval(a[..d], x) == polyval(a[..d'], x) + a[d'] * pow(x, d');
-        assert polyseg(a, x, 0, d) == polyseg(a, x, 0, d') + pow(x, d') * a[d'];
-
-        polyseg_equals_polyval_general(a, x, d');
-        assert polyval(a[..d'], x) == polyseg(a, x, 0, d');
+        calc {
+            pow(x, b);
+            == //Def. pow for n := b
+            x * pow(x, b - 1);
+            == {PowProperty(x, a, b-1);}
+            x * (pow(x, a) * pow(x, b - a - 1));
+            == //Rearrange
+            pow(x, a) * x * pow(x, b - a - 1);
+            == //Def. pow for n := b - 1
+            pow(x, a) * pow(x, b - a);
+        }
     }
 }
 
-lemma polyseg_equals_polyval(a: seq<int>, x:int)
-    ensures polyval(a, x) == polyseg(a, x, 0, |a|)
+lemma polyval_double_slicing(a: seq<int>, x:int, i:nat, j: nat) 
+    requires 0 <= i < j <= |a|
+    ensures polyval(a[i..j], x) == polyval(a[i..j-1], x) + a[j-1] * pow(x, j-i-1)
 {
-    polyseg_equals_polyval_general(a, x, |a|);
-    assert polyval(a[..|a|], x) == polyseg(a, x, 0, |a|);
-    assert a[..|a|] == a;
+    // Step 1: Show that a[i..j] is the concatenation of a[i..j-1] and [a[j-1]]
+    assert a[i..j] == a[i..j-1] + [a[j-1]];
+
+    // Step 2: Apply the definition of polyval to a[i..j]
+    var d := |a[i..j]| - 1; // Degree of the polynomial
+    assert d == j - i - 1; // Since |a[i..j]| = j - i
+
+    // Step 3: Expand polyval(a[i..j], x) using its definition
+    assert polyval(a[i..j], x) == polyval(a[i..j-1], x) + a[j-1] * pow(x, d);
+
+    // Step 4: Substitute d = j - i - 1
+    assert polyval(a[i..j], x) == polyval(a[i..j-1], x) + a[j-1] * pow(x, j-i-1);
+
+}
+
+function polyseg(a: seq<int>, x: int, lo: nat, hi: nat): int
+  requires hi <= |a| && |a| > lo >= 0 && lo < hi // Ensure hi is within bounds
+  ensures polyseg(a, x, lo, hi) == pow(x, lo) * polyval(a[lo..hi], x) // Postcondition
+{
+  if lo >= hi-1 then
+    var res := a[lo] * pow(x, lo);
+    res
+  else 
+    var r := polyseg(a, x, lo, hi-1);
+    var res := r + a[hi-1] * pow(x, hi-1);
+    calc{
+        res;
+        == //Def. res
+        r + a[hi-1] * pow(x, hi-1);
+        == //Def. r
+        polyval(a[lo..hi-1], x) * pow(x, lo) + a[hi-1] * pow(x, hi-1);
+        == {PowProperty(x, lo, hi - 1);}
+        pow(x, lo) * (polyval(a[lo..hi-1], x) + a[hi-1] * pow(x, hi-lo-1));
+        == {polyval_double_slicing(a, x, lo, hi);}
+        pow(x, lo) * polyval(a[lo..hi], x);
+    }
+    res
+}
+
+lemma polyseg_Equals_Polyval(a: seq<int>, x:int) 
+    requires |a| > 0
+    ensures polyseg(a, x, 0, |a|) == polyval(a, x)
+{
+    assert polyseg(a, x, 0, |a|) == polyval(a, x);
+}
+
+lemma polyseg_decomposition(a: seq<int>, x: int, lo: nat, hi: nat)
+  requires hi <= |a| && |a| > lo >= 0 && lo < hi - 1 // Ensure hi is within bounds
+  ensures polyseg(a, x, lo, hi) == a[lo] * pow(x, lo) + polyseg(a, x, lo+1, hi)
+{
+    if lo == hi - 2 {
+        assert hi == lo + 2;
+        assert polyseg(a, x, lo, lo+2) == a[lo] * pow(x, lo) + polyseg(a, x, lo+1, lo+2);
+    } else {
+        calc {
+            polyseg(a, x, lo, hi);
+            == //Def. polyseg
+            polyseg(a, x, lo, hi-1) + a[hi-1] * pow(x, hi-1);
+            == {polyseg_decomposition(a, x, lo, hi - 1);}
+            a[lo] * pow(x, lo) + polyseg(a, x, lo+1, hi - 1) + a[hi-1] * pow(x, hi-1);
+            ==
+            a[lo] * pow(x, lo) + polyseg(a, x, lo+1, hi);
+        }
+    }
 }
 // END-TODO(Optional)
 
@@ -134,5 +186,36 @@ method polyPowerCache(a: seq<int>, x: int) returns (r: int)
 method Horner(a: seq<int>, x: int) returns (r: int)
     ensures r == polyval(a, x)
 // BEGIN-TODO(HornerPoly)
-// Implement Horner's scheme for calculating the value of a polynomial.
+{
+    if |a| == 0 {
+        r := 0;
+    } else {
+        var i := |a|-1;
+        r := a[i];
+        while i > 0 
+            invariant 0 <= i < |a|
+            invariant r * pow(x, i) == polyseg(a, x, i, |a|)
+            decreases i
+        {
+            //keep old variable to prove maintenance more easily
+            var r_old := r;
+
+            i := i - 1;
+            r := a[i] + x * r;
+            
+            //proof maintenance
+            calc {
+                r * pow(x, i);
+                ==
+                (a[i] + x * r_old) * pow(x, i);
+                ==
+                a[i] * pow(x, i) + x * pow(x, i) * r_old;
+                == {assert pow(x, i + 1) * r_old == polyseg(a, x, i + 1, |a|);}
+                a[i] * pow(x, i) + polyseg(a, x, i + 1, |a|);
+                == {polyseg_decomposition(a, x, i, |a|);}
+                polyseg(a, x, i, |a|);
+            }
+        }
+    }
+}
 // END-TODO(HornerPoly)
